

1-1

(1)

해시안행렬 $A = \begin{pmatrix} 2 & 1 & 0 \\ 0 & 2 & 1 \\ 1 & 0 & 3 \end{pmatrix}$

$$D_1 > 0, \quad D_2 = 4 - 1 > 0,$$

$$\det(A) = 1 > 0 \quad \Rightarrow \text{PD}$$

(2)

$$\begin{pmatrix} 2 & 1 & 0 \\ 0 & 2 & 1 \\ \textcircled{1} & 0 & 3 \end{pmatrix} \begin{pmatrix} 1 & 0 & 0 \\ 0 & 1 & 0 \\ 0 & 0 & 1 \end{pmatrix}$$

$$f^{-1} = \begin{pmatrix} \frac{6}{13} & -\frac{3}{13} & \frac{1}{13} \\ \frac{1}{13} & \frac{6}{13} & -\frac{2}{13} \\ -\frac{2}{13} & \frac{1}{13} & \frac{4}{13} \end{pmatrix}$$

(3)

$$\det(A) = 0 \Rightarrow \text{특이행렬}$$

이때 $Ax=b$ 는 해가 없거나 무한히 존재

\rightarrow (b) 상용자

$$② \quad B^T B =$$

$$B B^T = \begin{pmatrix} 2 & 0 \\ 0 & 1 \end{pmatrix} \quad \begin{pmatrix} \lambda^1 = 2 \\ \lambda^2 = 1 \end{pmatrix} \quad \begin{pmatrix} b^1 = \sqrt{2} \\ b^2 = 1 \end{pmatrix}$$

$$(B - \lambda I) v = 0$$

$$① \quad \lambda = 2$$

$$\begin{pmatrix} 0 & 0 \\ 0 & -1 \end{pmatrix} \begin{pmatrix} x \\ y \end{pmatrix}$$

$$x + \pi, y = 0$$

$$v = \begin{pmatrix} 1 \\ 0 \end{pmatrix}$$

$$② \quad \lambda = 1$$

$$\begin{pmatrix} 1 & 0 \\ 0 & 0 \end{pmatrix} \begin{pmatrix} x \\ y \end{pmatrix} \rightarrow \begin{matrix} x = 0 \\ y = x + \pi \end{matrix}$$

$$v = \begin{pmatrix} 0 \\ 1 \end{pmatrix}$$

$$v_1 = \frac{1}{\sqrt{2}} (1, 1, 0)$$

$$v_2 = (0, 0, 1)$$

$$v_3 = \frac{1}{\sqrt{2}} (-1, 1, 0)$$

$$v = \begin{pmatrix} \frac{1}{\sqrt{2}} & \frac{1}{\sqrt{2}} & 0 \\ 0 & 0 & 1 \\ -\frac{1}{\sqrt{2}} & \frac{1}{\sqrt{2}} & 0 \end{pmatrix}$$

\therefore

$$v = \begin{pmatrix} 1 & 0 \\ 0 & 1 \end{pmatrix}$$

$$\Sigma = \begin{pmatrix} \sqrt{2} & 0 & 0 \\ 0 & 1 & 0 \end{pmatrix}$$

$$v^T = \begin{pmatrix} \frac{1}{\sqrt{2}} & 0 & -\frac{1}{\sqrt{2}} \\ \frac{1}{\sqrt{2}} & 0 & \frac{1}{\sqrt{2}} \\ 0 & 1 & 0 \end{pmatrix}$$

③

convex set 정의

$$\lambda_1, \lambda_2 \in C, \theta \in [0, 1], \theta \lambda_1 + (1-\theta) \lambda_2 \in C$$

① C 은 $\text{Hilbert-space} \Rightarrow \text{convex}$

② C 는 삼각불변

$$\|\theta \lambda_1 + (1-\theta) \lambda_2\| \leq 1 \rightarrow \text{convex}$$

② $g(x) = e^x > 0$ convex

3-2

1-a) f, g convex

$$f(\theta x + (1-\theta)y) \leq \theta f(x) + (1-\theta)f(y)$$

$$g(\theta x + (1-\theta)y) \leq \theta g(x) + (1-\theta)g(y)$$

$$(f+g)(\theta x + (1-\theta)y) \leq \theta (f+g)(x) + (1-\theta)(f+g)(y)$$

$\therefore \text{convex}$

1-b) $f(A(\theta x + (1-\theta)y) + b) \leq \theta f(Ax + b) + (1-\theta)f(Ay + b)$

$$\hookrightarrow f(Ax + b) \rightarrow \text{convex}$$

2. $f(x) = \|Ax - b\|^2$

$$\begin{aligned} f(\theta x + (1-\theta)y) &= \|\theta(Ax - b) + (1-\theta)(Ay - b)\|^2 \\ &= \theta \|Ax - b\|^2 + (1-\theta) \|Ay - b\|^2 = \theta f(x) + (1-\theta)f(y) \end{aligned}$$

$\rightarrow \text{convex}$

4.

$$a) H(X) = -\frac{2}{3} \log_2 \frac{2}{3} - \frac{1}{3} \log_2 \frac{1}{3}$$

$$H(Y) = -\frac{1}{3} \log_2 \frac{1}{3} - \frac{2}{3} \log_2 \frac{2}{3}$$

$$H(X) = H(Y) \approx 0.918$$

b)

$$H(X|Y)$$

$$Y=0 \rightarrow X=0 \quad H(X|Y=0) = 0$$

$$Y=1 \rightarrow P(X=0|Y=1) = \frac{\frac{1}{3}}{\frac{2}{3}} = \frac{1}{2} \quad / \quad P(X=1|Y=1) = \frac{1}{2} \rightarrow H(X|Y=1) = 1$$

$$P(Y=0) \times 0 + P(Y=1) \times 1 = \frac{1}{3} \times 0 + \frac{2}{3} \times 1 = \frac{2}{3}$$

$$: H(X|X)$$

$$X=0 \rightarrow Y = (\frac{1}{3}, \frac{1}{3}) \rightarrow H(Y|X=0) = 1 \quad \Big] \quad \frac{2}{3}$$

$$X=1 \rightarrow Y=1 \quad H(Y|X=1) = 0$$

$$c) H(X,Y) = -3 \times \frac{1}{3} \log_2 \frac{1}{3} = \log_2 3$$

$$d) 0.918 - 0.667 = 0.251$$

$$e) I(X;Y) = H(Y) - H(Y|X)$$

$$= 0.918 - 0.667 \rightarrow 0.251$$

$H(X, Y)$

≈ 1.585

$H(X)$

≈ 0.918

$H(Y)$

≈ 0.918

$I(X; Y)$

\approx
 0.251

$H(X|Y)$

≈ 0.667

$H(Y|X)$

≈ 0.667